Source/DafnyCore/AST/Members/SpecialField.cs
@@ -59,26 +59,17 @@ public class SpecialField : Field {
     }
   }
 
-  public override string FullSanitizedName { // Override beacuse EnclosingClass may be null
+  public override string FullSanitizedName { // Override because EnclosingClass may be null
     get {
       Contract.Ensures(Contract.Result<string>() != null);
-      return EnclosingClass != null ? 
-        EnclosingClass.FullSanitizedName + "." + 
-        (EnclosingMethod != null ?
-          EnclosingMethod.FullSanitizedName + "." +
-          (AtCallSite ? "call." : "")
-          : "")
-        + SanitizedName : SanitizedName;
+      return EnclosingMethod != null ? EnclosingMethod.FullSanitizedName + "." + SanitizedName
+        : EnclosingClass != null ? EnclosingClass.FullSanitizedName + "." + SanitizedName : SanitizedName;
     }
   }
 
   // Used by referrers to designate the memory location of local variables and method parameters
   [FilledInDuringResolution]
   [CanBeNull] public MethodOrConstructor EnclosingMethod { get; set; }
-  
-  // Used by referrers to designate if the memory location of input parameters is a call site or in the body of a method
-  [FilledInDuringResolution]
-  [CanBeNull] public bool AtCallSite { get; set; }
 
   public override string GetCompileName(DafnyOptions options) {
     Contract.Ensures(Contract.Result<string>() != null);
